feat: prove states lt array size

Regex/Compiler.lean
@@ -1,6 +1,11 @@
+import Init.Meta
 import Batteries.Data.Array.Basic
+import Batteries.Lean.Except
+
 import Regex.Syntax.Hir
 import Regex.Nfa
+import Regex.Tactic.SimpLte
+import Regex.Data.Nat.Basic
 
 namespace Compiler
 
@@ -20,8 +25,10 @@ structure Config where
   unanchored_prefix: Bool
   /-- Whether to simulate an unanchored prefix with the backtracker. -/
   unanchored_prefix_simulation : Bool
+  /-- Max recurciosn deth in compilation -/
+  fuel : Nat
 
-instance : Inhabited Config := ⟨⟨true, false⟩⟩
+instance : Inhabited Config := ⟨⟨true, false, 1000⟩⟩
 
 /-- A value that represents the result of compiling a sub-expression of a regex's HIR.
     Specifically, this represents a sub-graph of the NFA that
@@ -31,211 +38,430 @@ structure ThompsonRef where
   start: Unchecked.StateID
   «end»: Unchecked.StateID
 
-instance : Inhabited ThompsonRef := ⟨0, 0⟩
-
 instance : ToString ThompsonRef where
   toString s := s!"{s.start}, {s.end}"
 
-abbrev CompilerM := StateT (Array Unchecked.State × Array Nat) (Except String)
+abbrev States := { a : Array Unchecked.State // ∀ i (h : i < a.size), (a.get i h).nextOf < a.size }
+
+abbrev States' (states : States) :=
+  { states' : States // states.val.size ≤ states'.val.size}
+
+abbrev StateIDStates (states : States) :=
+  { pairs : Unchecked.StateID × States
+    // pairs.1 < pairs.2.val.size ∧ states.val.size < pairs.2.val.size}
+
+abbrev StateIDStates' (states states' : States) :=
+  { pairs : Unchecked.StateID × States
+    // pairs.1 < pairs.2.val.size ∧ states.val.size < pairs.2.val.size
+       ∧ states'.val.size ≤ pairs.2.val.size}
+
+abbrev ThompsonRefStates (states : States) :=
+  { pairs : ThompsonRef × States
+    // pairs.1.start < pairs.2.val.size ∧ pairs.1.«end» < pairs.2.val.size
+       ∧ states.val.size < pairs.2.val.size }
+
+def ThompsonRefStates.mk {states : States} (arg1Start arg1End : Unchecked.StateID) (arg2 : States)
+  (h : arg1Start < arg2.val.size
+        ∧ arg1End < arg2.val.size
+        ∧ states.val.size < arg2.val.size)
+    : ThompsonRefStates states :=
+  ⟨(⟨arg1Start, arg1End⟩ , arg2), h⟩
+
+def ThompsonRefStates.castLt {states states' : States} (t : ThompsonRefStates states)
+  (h : states'.val.size < t.val.snd.val.size) : ThompsonRefStates states' :=
+  ThompsonRefStates.mk t.val.1.start t.val.1.end t.val.2 (by
+    have ht := t.property
+    exact And.intro ht.left (And.intro ht.right.left h))
+
+abbrev CompilerM := StateT (Array Nat) (Except String)
+
+private theorem all_set {n : Unchecked.StateID} {s : Unchecked.State} {states : States}
+  (h : n < states.val.size) (hn : Unchecked.State.nextOf s < states.val.size)
+    : ∀ i (_ : i < (states.val.set n s h).size),
+     ((states.val.set n s h)[i].nextOf < (states.val.set n s h).size) := by
+  have hs := Array.size_set states.val n s h
+  intro i hi
+  rw [hs]
+  rw [hs] at hi
+  have := Array.getElem_set states.val n h s i (by rw [hs]; exact hi)
+  split at this
+  simp_all
+  rw [this]
+  exact states.property i hi
+
+private theorem all_push {s : Unchecked.State} {states : States}
+  (h : Unchecked.State.nextOf s ≤ states.val.size)
+    : ∀ i (_ : i < (states.val.push s).size),
+      ((states.val.push s)[i].nextOf < (states.val.push s).size) := by
+  intro i hi
+  have := Array.getElem_push states.val s i hi
+  simp_all
+  split
+  . rename_i h'
+    exact Nat.lt_add_right 1 (states.property i h')
+  . exact Nat.lt_add_one_of_le h
+
+private theorem eat_until_lt {states : States} (h : «from» < states.val.size)
+  (hm : states.val.get «from» h = Unchecked.State.Eat (Unchecked.EatMode.Until s) n)
+    : s < states.val.size ∧ n < states.val.size := by
+  have := states.property «from» h
+  rw [hm] at this
+  simp +zetaDelta [Unchecked.State.nextOf, Nat.max, @Nat.max_def s n] at this
+  exact Nat.max_lt.mp this
+
+private theorem eat_toLast_lt {states : States} (h : «from» < states.val.size)
+  (hm : states.val.get «from» h = Unchecked.State.Eat (Unchecked.EatMode.ToLast s) n)
+    : s < states.val.size ∧ n < states.val.size := by
+  have := states.property «from» h
+  rw [hm] at this
+  simp +zetaDelta [Unchecked.State.nextOf, Nat.max, @Nat.max_def s n] at this
+  exact Nat.max_lt.mp this
+
+private theorem change_frame_step_lt {states : States} (h : «from» < states.val.size)
+  (hm : states.val.get «from» h = Unchecked.State.ChangeFrameStep f t)
+    : f < states.val.size ∧ t < states.val.size := by
+  have := states.property «from» h
+  rw [hm] at this
+  simp +zetaDelta [Unchecked.State.nextOf, Nat.max, Nat.max_lt] at this
+  assumption
+
+private theorem binary_union_lt {states : States} (h : «from» < states.val.size)
+  (hm : states.val.get «from» h = Unchecked.State.BinaryUnion alt1 alt2)
+    : alt1 < states.val.size ∧ alt2 < states.val.size := by
+  have := states.property «from» h
+  rw [hm] at this
+  simp +zetaDelta [Unchecked.State.nextOf, Nat.max, Nat.max_lt] at this
+  assumption
+
+private theorem union_lt {states : States} (h : «from» < states.val.size)
+  (ht : to < states.val.size) (hm : states.val.get «from» h = Unchecked.State.Union alternates)
+    : List.maxD 0 (alternates.toList ++ [to]) < states.val.size := by
+  have := states.property «from» h
+  rw [hm] at this
+  simp +zetaDelta [Unchecked.State.nextOf] at this
+  exact List.maxD_of_append_lt this ht
+
+private theorem union_reverse_lt {states : States} (h : «from» < states.val.size)
+  (ht : to < states.val.size)
+  (hm : states.val.get «from» h = Unchecked.State.UnionReverse alternates)
+    : List.maxD 0 (alternates.toList ++ [to]) < states.val.size := by
+  have := states.property «from» h
+  rw [hm] at this
+  simp +zetaDelta [Unchecked.State.nextOf] at this
+  exact List.maxD_of_append_lt this ht
 
 /-- Add a transition from one state to another. -/
-private def patch («from» «to» : Unchecked.StateID) : CompilerM PUnit := do
-  let (states, groups) ← get
-  if h : «from» < states.size
-  then
-    match states.get «from» h with
-    | .Empty _ =>  set (states.set «from» (Unchecked.State.Empty «to») h, groups)
-    | .NextChar offset _ =>  set (states.set «from» (Unchecked.State.NextChar offset «to») h, groups)
-    | .Fail =>  Except.error s!"patch states .Fail unexpected"
-    | .Eat (.Until s) n =>
-        if s = 0 then set (states.set «from» (Unchecked.State.Eat (.Until «to») n) h, groups)
-        else if n = 0 then set (states.set «from» (Unchecked.State.Eat (.Until s) «to») h, groups)
-        else Except.error "patch states, .Eat s and n not null"
-    | .Eat (.ToLast s) n =>
-        if s = 0 then set (states.set «from» (Unchecked.State.Eat (.ToLast «to») n) h, groups)
-        else if n = 0 then set (states.set «from» (Unchecked.State.Eat (.ToLast s) «to») h, groups)
-        else Except.error "patch states, .Eat s and n not null"
-    | .ChangeFrameStep f t =>
-        if f = 0 then set (states.set «from» (Unchecked.State.ChangeFrameStep «to» t) h, groups)
-        else if t = 0 then set (states.set «from» (Unchecked.State.ChangeFrameStep f «to»), groups)
-        else Except.error "patch states, .ChangeFrameStep from and to not null"
-    | .RemoveFrameStep _ =>  set (states.set «from» (Unchecked.State.RemoveFrameStep «to») h, groups)
-    | .Look look _ =>  set (states.set «from» (Unchecked.State.Look look «to»), groups)
-    | .BackRef b f _ =>  set (states.set «from» (Unchecked.State.BackRef b f «to»), groups)
-    | .ByteRange t =>
-        set (states.set «from» (Unchecked.State.ByteRange {t with «next» := «to»}) h, groups)
-    | .Capture role _ pattern_id group_index slot =>
-        set (states.set «from» (Unchecked.State.Capture role «to» pattern_id group_index slot), groups)
-    | .BinaryUnion alt1 alt2 =>
-        if alt1 = 0 then set (states.set «from» (Unchecked.State.BinaryUnion «to» alt2) h, groups)
-        else if alt2 = 0 then set (states.set «from» (Unchecked.State.BinaryUnion alt1 «to») h, groups)
-        else Except.error "patch states, .BinaryUnion alt1 and alt2 not null"
-    | .SparseTransitions _ => set (states, groups) -- todo
-    | .Union alternates =>
-        set (states.set «from» (Unchecked.State.Union (alternates.push «to»)) h, groups)
-    | .UnionReverse alternates =>
-        set (states.set «from» (Unchecked.State.UnionReverse (alternates.push «to»)) h, groups)
-    | .Match _ => Except.error s!"patch states .Match unexpected"
-  else  Except.error s!"patch not valid, {«from»} ge size {states.size}"
+private def patch («from» «to» : Unchecked.StateID) (states : States)
+  (ht : «to» < states.val.size) (h : «from» < states.val.size)
+    : CompilerM { states' : States // states.val.size = states'.val.size } := do
+  match hm : states.val.get «from» h with
+  | .Empty _ =>
+    have hn : (Unchecked.State.Empty «to»).nextOf = «to» := by
+      simp +zetaDelta [Unchecked.State.nextOf]
+    pure ⟨⟨states.val.set «from» (Unchecked.State.Empty «to») h, all_set h (by simp [hn, ht])⟩,
+          by simp_all⟩
+  | .NextChar offset _ =>
+    pure ⟨⟨states.val.set «from» (Unchecked.State.NextChar offset «to») h, by
+            apply all_set; simp +zetaDelta [Unchecked.State.nextOf, ht]⟩,
+          by simp_all⟩
+  | .Fail =>  Except.error s!"patch states .Fail unexpected"
+  | .Eat (.Until s) n =>
+      if s = 0
+      then pure ⟨⟨states.val.set «from» (Unchecked.State.Eat (.Until «to») n) h, by
+                  apply all_set
+                  simp +zetaDelta [Unchecked.State.nextOf, ht, Nat.max_lt, eat_until_lt h hm]⟩,
+                by simp_all⟩
+      else if n = 0
+      then pure ⟨⟨states.val.set «from» (Unchecked.State.Eat (.Until s) «to») h, by
+                  apply all_set
+                  simp +zetaDelta [Unchecked.State.nextOf, ht, Nat.max_lt, eat_until_lt h hm]⟩,
+                by simp_all⟩
+      else Except.error "patch states, .Eat s and n not null"
+  | .Eat (.ToLast s) n =>
+      if s = 0
+      then pure ⟨⟨states.val.set «from» (Unchecked.State.Eat (.ToLast «to») n) h, by
+                  apply all_set
+                  simp +zetaDelta [Unchecked.State.nextOf, ht, Nat.max_lt, eat_toLast_lt h hm]⟩,
+                by simp_all⟩
+      else if n = 0 then
+      pure ⟨⟨states.val.set «from» (Unchecked.State.Eat (.ToLast s) «to») h, by
+                  apply all_set
+                  simp +zetaDelta [Unchecked.State.nextOf, ht, Nat.max_lt, eat_toLast_lt h hm]⟩,
+                by simp_all⟩
+      else Except.error "patch states, .Eat s and n not null"
+  | .ChangeFrameStep f t =>
+      if f = 0
+      then pure ⟨⟨states.val.set «from» (Unchecked.State.ChangeFrameStep «to» t) h, by
+                  apply all_set; simp +zetaDelta [Unchecked.State.nextOf,
+                    change_frame_step_lt h hm, Nat.max_lt, ht]⟩,
+        by simp_all⟩
+      else if t = 0
+      then pure ⟨⟨states.val.set «from» (Unchecked.State.ChangeFrameStep f «to»), by
+                  apply all_set
+                  simp +zetaDelta [Unchecked.State.nextOf, change_frame_step_lt h hm,
+                                    Nat.max_lt, ht]⟩,
+                by simp_all⟩
+      else Except.error "patch states, .ChangeFrameStep from and to not null"
+  | .RemoveFrameStep _ =>
+    pure ⟨⟨states.val.set «from» (Unchecked.State.RemoveFrameStep «to») h, by
+            apply all_set; simp +zetaDelta [Unchecked.State.nextOf, ht]⟩,
+          by simp_all⟩
+  | .Look look _ =>
+    pure ⟨⟨states.val.set «from» (Unchecked.State.Look look «to»), by
+            apply all_set; simp +zetaDelta [Unchecked.State.nextOf, ht]⟩,
+          by simp_all⟩
+  | .BackRef b f _ =>
+    pure ⟨⟨states.val.set «from» (Unchecked.State.BackRef b f «to»), by
+            apply all_set; simp +zetaDelta [Unchecked.State.nextOf, ht, Nat.zero_lt_of_lt ht]⟩,
+          by simp_all⟩
+  | .ByteRange t =>
+      pure ⟨⟨states.val.set «from» (Unchecked.State.ByteRange {t with «next» := «to»}) h, by
+              apply all_set; simp +zetaDelta [Unchecked.State.nextOf, ht]⟩,
+            by simp_all⟩
+  | .Capture role _ pattern_id group_index slot =>
+      pure ⟨⟨states.val.set «from» (Unchecked.State.Capture role «to» pattern_id group_index slot),
+              by apply all_set; simp +zetaDelta [Unchecked.State.nextOf, ht, Nat.zero_lt_of_lt ht]⟩,
+            by simp_all⟩
+  | .BinaryUnion alt1 alt2 =>
+      if alt1 = 0
+      then pure ⟨⟨states.val.set «from» (Unchecked.State.BinaryUnion «to» alt2) h, by
+                  apply all_set; simp +zetaDelta [Unchecked.State.nextOf,
+                        binary_union_lt h hm, Nat.max_lt, ht]⟩,
+                by simp_all⟩
+      else if alt2 = 0
+      then pure ⟨⟨states.val.set «from» (Unchecked.State.BinaryUnion alt1 «to») h, by
+                  apply all_set; simp +zetaDelta [Unchecked.State.nextOf,
+                        binary_union_lt h hm, Nat.max_lt, ht]⟩,
+                by simp_all⟩
+      else Except.error "patch states, .BinaryUnion alt1 and alt2 not null"
+  | .SparseTransitions _ => pure ⟨(states), by simp_all⟩
+  | .Union alternates =>
+      pure ⟨⟨states.val.set «from» (Unchecked.State.Union (alternates.push «to»)) h, by
+              apply all_set; simp +zetaDelta [Unchecked.State.nextOf, union_lt h ht hm]⟩,
+            by simp_all⟩
+  | .UnionReverse alternates =>
+      pure ⟨⟨states.val.set «from» (Unchecked.State.UnionReverse (alternates.push «to»)) h, by
+              apply all_set; simp +zetaDelta [Unchecked.State.nextOf, union_reverse_lt h ht hm]⟩,
+            by simp_all⟩
+  | .Match _ => Except.error s!"patch states .Match unexpected"
 
-private def push (s : Unchecked.State) : CompilerM Unchecked.StateID := do
-  let (states, groups) ← get
-  set (states.push s, groups)
-  pure states.size
+private def push (s : Unchecked.State) (states : States)
+  (h : NFA.Unchecked.State.nextOf s ≤ states.val.size) : CompilerM (StateIDStates states) := do
+  pure ⟨(states.val.size, ⟨states.val.push s, all_push h⟩), by simp_all⟩
 
-private def push' (s : Unchecked.State) : CompilerM ThompsonRef := do
-  let (states, groups) ← get
-  set (states.push s, groups)
-  pure ⟨states.size, states.size⟩
+private def push' (s : Unchecked.State) (states : States)
+  (h : NFA.Unchecked.State.nextOf s ≤ states.val.size) : CompilerM (ThompsonRefStates states) := do
+  pure ⟨(⟨states.val.size, states.val.size⟩, ⟨states.val.push s, all_push h⟩),
+        by exact And.intro (by simp_all) (by simp_all)⟩
 
-private def add_match (pattern_id : PatternID) : CompilerM Unchecked.StateID :=
-  push (Unchecked.State.Match pattern_id)
+private def add_match (pattern_id : PatternID) (states : States)
+    : CompilerM (StateIDStates states) :=
+  push (Unchecked.State.Match pattern_id) states (by
+    simp +zetaDelta [Unchecked.State.nextOf])
 
-private def add_union : CompilerM Unchecked.StateID :=
-  push (Unchecked.State.Union #[])
+private def add_union (states : States) : CompilerM (StateIDStates states) :=
+  push (Unchecked.State.Union #[]) states (by
+    simp_all +zetaDelta [Unchecked.State.nextOf, List.maxD_of_empty_eq])
 
-private def add_union_reverse : CompilerM Unchecked.StateID  :=
-  push (Unchecked.State.UnionReverse #[])
+private def add_union_reverse (states : States) : CompilerM (StateIDStates states) :=
+  push (Unchecked.State.UnionReverse #[]) states (by
+    simp_all +zetaDelta [Unchecked.State.nextOf, List.maxD_of_empty_eq])
 
-private def add_backrefence (case_insensitive : Bool) (b : Nat)  : CompilerM Unchecked.StateID :=
-  push (Unchecked.State.BackRef b case_insensitive 0)
+private def add_backrefence (case_insensitive : Bool) (b : Nat) (states : States)
+    : CompilerM (StateIDStates states) :=
+  push (Unchecked.State.BackRef b case_insensitive 0) states (by
+    simp_all +zetaDelta [Unchecked.State.nextOf])
 
-private def c_range (start «end» : UInt32) : CompilerM ThompsonRef :=
+private def c_range (start «end» : UInt32) (states : States)
+    : CompilerM (ThompsonRefStates states) :=
   let trans: Unchecked.Transition := ⟨start, «end», 0⟩
-  push' (Unchecked.State.ByteRange trans)
+  push' (Unchecked.State.ByteRange trans) states (by simp_all +zetaDelta [Unchecked.State.nextOf])
 
-private def add_empty : CompilerM Unchecked.StateID  :=
-  push (Unchecked.State.Empty 0)
+private def add_empty (states : States) : CompilerM (StateIDStates states)  :=
+  push (Unchecked.State.Empty 0) states (by simp +zetaDelta [Unchecked.State.nextOf])
 
-private def add_fail  : CompilerM Unchecked.StateID :=
-  push (Unchecked.State.Fail)
+private def add_fail (states : States) : CompilerM (StateIDStates states) :=
+  push (Unchecked.State.Fail) states (by simp +zetaDelta [Unchecked.State.nextOf])
 
-private def add_eat (mode : Unchecked.EatMode) : CompilerM Unchecked.StateID :=
-  push (Unchecked.State.Eat mode 0)
+private def add_eat (mode : Unchecked.EatMode) (states : States) (h : mode.nextOf ≤ states.val.size)
+    : CompilerM (StateIDStates states) :=
+  push (Unchecked.State.Eat mode 0) states (by
+    simp +zetaDelta [Unchecked.State.nextOf]
+    split <;> try simp_all
+    · rename_i s next heq
+      simp_all [Nat.max_le]
+      rw [← heq.right]
+      simp [Unchecked.EatMode.nextOf] at h
+      exact And.intro (by assumption) (by exact Nat.zero_le states.val.size)
+    · rename_i s next heq
+      simp_all [Nat.max_le]
+      rw [← heq.right]
+      simp [Unchecked.EatMode.nextOf] at h
+      exact And.intro (by assumption) (by exact Nat.zero_le states.val.size))
 
-private def add_change_state : CompilerM Unchecked.StateID  :=
-  push (Unchecked.State.ChangeFrameStep 0 0)
+private def add_change_state (states : States) : CompilerM (StateIDStates states) :=
+  push (Unchecked.State.ChangeFrameStep 0 0) states (by simp +zetaDelta [Unchecked.State.nextOf])
 
-private def add_remove_state : CompilerM Unchecked.StateID  :=
-  push (Unchecked.State.RemoveFrameStep 0)
+private def add_remove_state (states : States) : CompilerM (StateIDStates states) :=
+  push (Unchecked.State.RemoveFrameStep 0) states (by simp +zetaDelta [Unchecked.State.nextOf])
 
-private def add_next_char (offset : Nat) : CompilerM Unchecked.StateID  :=
-  push (Unchecked.State.NextChar offset 0)
+private def add_next_char (offset : Nat) (states : States) : CompilerM (StateIDStates states) :=
+  push (Unchecked.State.NextChar offset 0) states (by simp +zetaDelta [Unchecked.State.nextOf])
 
-private def c_empty : CompilerM ThompsonRef :=
-  push' (Unchecked.State.Empty 0)
+private def c_empty (states : States) : CompilerM (ThompsonRefStates states) :=
+  push' (Unchecked.State.Empty 0) states (by simp +zetaDelta [Unchecked.State.nextOf])
 
-private def add_sparse (trans : Array Unchecked.Transition) : CompilerM Unchecked.StateID  :=
-  push (Unchecked.State.SparseTransitions trans)
+private def add_sparse (trans : Array Unchecked.Transition) (states : States)
+  (h : ∀ (i) (h : i < trans.size), (trans.get i h).next ≤ states.val.size)
+    : CompilerM (StateIDStates states)  :=
+  push (Unchecked.State.SparseTransitions trans) states (by
+    simp +zetaDelta [Unchecked.State.nextOf]
+    have h : ∀ a ∈ trans.toList, a.next ≤ states.val.size := by
+      intro a ha
+      have ha : a ∈ trans := Array.mem_def.mpr ha
+      have ⟨i, ⟨hlt, heq⟩⟩ := Array.mem_iff_getElem.mp ha
+      have := h i hlt
+      simp_all
+    exact List.maxD_of_all_map_le h)
 
-private def c_unicode_class (cls : ClassUnicode) : CompilerM ThompsonRef := do
-  let «end» ← add_empty
-  let trans : Array Unchecked.Transition :=
-    cls.set.intervals.map (fun r => ⟨r.fst.val, r.snd.val, «end»⟩)
-  let start ← add_sparse trans
-  pure ⟨start, «end»⟩
+private def c_unicode_class (cls : ClassUnicode) (states : States)
+    : CompilerM (ThompsonRefStates states) := do
+  let «end» ← add_empty states
+  let f : NonemptyInterval Char→Unchecked.Transition := fun r => ⟨r.fst.val, r.snd.val, «end».val.1⟩
+  let trans : Array Unchecked.Transition := cls.set.intervals.map f
+  let start ← add_sparse trans «end».val.2 (by
+    intro i hi
+    have := Array.getElem?_map f cls.set.intervals i
+    simp_all +zetaDelta
+    exact Nat.le_of_succ_le «end».property.left)
+  pure (ThompsonRefStates.mk start.val.1 «end».val.1 start.val.2 (by
+    have ⟨_, _⟩ := «end».property
+    have ⟨_, _⟩ := start.property
+    and_intros <;> simp_lte))
 
-private def c_literal (c : Char) : CompilerM ThompsonRef :=
-  c_range c.val c.val
+private def c_literal (c : Char) (states : States) : CompilerM (ThompsonRefStates states) :=
+  c_range c.val c.val states
 
-private def c_look : Syntax.Look -> CompilerM ThompsonRef
-  | .Start => push' (Unchecked.State.Look NFA.Look.Start 0)
-  | .End => push' (Unchecked.State.Look NFA.Look.End 0)
-  | .EndWithOptionalLF => push' (Unchecked.State.Look NFA.Look.EndWithOptionalLF 0)
-  | .StartLF => push' (Unchecked.State.Look NFA.Look.StartLF 0)
-  | .EndLF => push' (Unchecked.State.Look NFA.Look.EndLF 0)
-  | .StartCRLF => push' (Unchecked.State.Look NFA.Look.StartCRLF 0)
-  | .EndCRLF => push' (Unchecked.State.Look NFA.Look.EndCRLF 0)
-  | .WordUnicode => push' (Unchecked.State.Look NFA.Look.WordUnicode 0)
-  | .WordUnicodeNegate => push' (Unchecked.State.Look NFA.Look.WordUnicodeNegate 0)
-  | .WordStartUnicode => push' (Unchecked.State.Look NFA.Look.WordStartUnicode 0)
-  | .WordEndUnicode => push' (Unchecked.State.Look NFA.Look.WordEndUnicode 0)
-  | .WordStartHalfUnicode => push' (Unchecked.State.Look NFA.Look.WordStartHalfUnicode 0)
-  | .WordEndHalfUnicode => push' (Unchecked.State.Look NFA.Look.WordEndHalfUnicode 0)
-  | .PreviousMatch => push' (Unchecked.State.Look NFA.Look.PreviousMatch 0)
-  | .ClearMatches => push' (Unchecked.State.Look NFA.Look.ClearMatches 0)
+private def c_look (look : Syntax.Look) (states : States) : CompilerM (ThompsonRefStates states) :=
+  match look with
+  | .Start => push' (Unchecked.State.Look NFA.Look.Start 0) states
+      (by simp +zetaDelta [Unchecked.State.nextOf])
+  | .End => push' (Unchecked.State.Look NFA.Look.End 0) states
+      (by simp +zetaDelta [Unchecked.State.nextOf])
+  | .EndWithOptionalLF => push' (Unchecked.State.Look NFA.Look.EndWithOptionalLF 0) states
+      (by simp +zetaDelta [Unchecked.State.nextOf])
+  | .StartLF => push' (Unchecked.State.Look NFA.Look.StartLF 0) states
+      (by simp +zetaDelta [Unchecked.State.nextOf])
+  | .EndLF => push' (Unchecked.State.Look NFA.Look.EndLF 0) states
+      (by simp +zetaDelta [Unchecked.State.nextOf])
+  | .StartCRLF => push' (Unchecked.State.Look NFA.Look.StartCRLF 0) states
+      (by simp +zetaDelta [Unchecked.State.nextOf])
+  | .EndCRLF => push' (Unchecked.State.Look NFA.Look.EndCRLF 0) states
+      (by simp +zetaDelta [Unchecked.State.nextOf])
+  | .WordUnicode => push' (Unchecked.State.Look NFA.Look.WordUnicode 0) states
+      (by simp +zetaDelta [Unchecked.State.nextOf])
+  | .WordUnicodeNegate => push' (Unchecked.State.Look NFA.Look.WordUnicodeNegate 0) states
+      (by simp +zetaDelta [Unchecked.State.nextOf])
+  | .WordStartUnicode => push' (Unchecked.State.Look NFA.Look.WordStartUnicode 0) states
+      (by simp +zetaDelta [Unchecked.State.nextOf])
+  | .WordEndUnicode => push' (Unchecked.State.Look NFA.Look.WordEndUnicode 0) states
+      (by simp +zetaDelta [Unchecked.State.nextOf])
+  | .WordStartHalfUnicode => push' (Unchecked.State.Look NFA.Look.WordStartHalfUnicode 0) states
+      (by simp +zetaDelta [Unchecked.State.nextOf])
+  | .WordEndHalfUnicode => push' (Unchecked.State.Look NFA.Look.WordEndHalfUnicode 0) states
+      (by simp +zetaDelta [Unchecked.State.nextOf])
+  | .PreviousMatch => push' (Unchecked.State.Look NFA.Look.PreviousMatch 0) states
+      (by simp +zetaDelta [Unchecked.State.nextOf])
+  | .ClearMatches => push' (Unchecked.State.Look NFA.Look.ClearMatches 0) states
+      (by simp +zetaDelta [Unchecked.State.nextOf])
 
-private def c_cap' (role : Capture.Role) (pattern_id slot: Nat) : CompilerM Unchecked.StateID  :=
-  push (Unchecked.State.Capture role 0 0 pattern_id slot)
+private def c_cap' (role : Capture.Role) (pattern_id slot: Nat) (states : States)
+    : CompilerM (StateIDStates states)  :=
+  push (Unchecked.State.Capture role 0 0 pattern_id slot) states (by simp +zetaDelta [Unchecked.State.nextOf])
 
 mutual
 
-private def c_concat (hirs : Array Hir) : CompilerM ThompsonRef := do
+private def c_concat (hirs : Array Hir) (states : States) : CompilerM (ThompsonRefStates states) := do
   match h : hirs.head? with
   | some (head, tail) =>
     have : sizeOf head < sizeOf hirs := Array.sizeOf_head?_of_mem h
-    let ⟨start, «end»⟩ ← c head
-
+    let ⟨(⟨start, «end»⟩, states'), _⟩ ← c head states
     have : sizeOf tail < sizeOf hirs := Array.sizeOf_head?_of_tail h
-    let hir ← tail.attach.foldlM (init := «end»)
-      (fun s (h : { x // x ∈ tail}) => do
-        have : sizeOf h.val < sizeOf tail := Array.sizeOf_lt_of_mem h.property
-        let hir ← c h.val
-        patch s hir.start
-        pure hir.end)
+    let (⟨(hir, states''), _⟩ : (StateIDStates' states states')) ← tail.attach.foldlM
+      (init := ⟨(«end», states'), by simp_all⟩)
+      (fun ⟨(s, states), _⟩ ⟨hir, h⟩ => do
+        have : sizeOf hir < sizeOf tail := Array.sizeOf_lt_of_mem h
+        let ⟨(hir, states), _⟩ ← c hir states
+        let states ← patch s hir.start states (by simp_lte) (by simp_lte)
+        pure ⟨(hir.end, states), by and_intros <;> simp_lte⟩)
 
-    pure ⟨start, hir⟩
-  | none => c_empty
+    pure (ThompsonRefStates.mk start hir states'' (by and_intros <;> simp_lte))
+  | none => c_empty states
 termination_by sizeOf hirs
 
-private def c_alt_iter (hirs : Array Hir) : CompilerM ThompsonRef := do
+private def c_alt_iter (hirs : Array Hir) (states : States) : CompilerM (ThompsonRefStates states) := do
   match hHead : hirs.head? with
   | some (first, tail) =>
     have : sizeOf tail < sizeOf hirs := Array.sizeOf_head?_of_tail hHead
     match hTail : tail.head? with
     | some (second, tail') =>
       have : sizeOf first < sizeOf hirs := Array.sizeOf_head?_of_mem hHead
-      let first ← c first
+      let ⟨(first, states), _⟩ ← c first states
       have : sizeOf second < sizeOf tail := Array.sizeOf_head?_of_mem hTail
-      let second ← c second
-      let union ← add_union
-      let «end» ← add_empty
+      let ⟨(second, states), _⟩ ← c second states
+      let ⟨(union, states), _⟩ ← add_union states
+      let ⟨(«end», states), _⟩ ← add_empty states
 
-      patch union first.start
-      patch first.end «end»
-      patch union second.start
-      patch second.end «end»
+      let states ← patch union first.start states (by simp_lte) (by simp_lte)
+      let states ← patch first.end «end» states (by simp_lte) (by simp_lte)
+      let states ← patch union second.start states (by simp_lte) (by simp_lte)
+      let states ← patch second.end «end» states (by simp_lte) (by simp_lte)
 
       have : sizeOf tail' < sizeOf tail := Array.sizeOf_head?_of_tail hTail
-      tail'.attach.forM
-        (fun (h : { x // x ∈ tail'}) => do
-          have : sizeOf h.val < sizeOf tail' := Array.sizeOf_lt_of_mem h.property
-          let compiled ← c h.val
-          patch union compiled.start
-          patch compiled.end «end»)
+      let (⟨states', _⟩ : States' states) ← tail'.attach.foldlM (init := ⟨states, by simp_all⟩)
+        (fun ⟨states, _⟩ ⟨hir, h⟩  => do
+          have : sizeOf hir < sizeOf tail' := Array.sizeOf_lt_of_mem h
+          let ⟨(compiled, states), _⟩ ← c hir states
+          let states ← patch union compiled.start states (by simp_lte) (by simp_lte)
+          let states ← patch compiled.end «end» states (by simp_lte) (by simp_lte)
+          pure ⟨states, by simp_lte⟩)
 
-      pure ⟨union, «end»⟩
+      pure (ThompsonRefStates.mk union «end» states' (by and_intros <;> simp_lte))
     | none => Except.error "c_alt_iter, size > 1 expected"
   | none => Except.error "c_alt_iter, size > 0 expected"
 termination_by sizeOf hirs
 
-private def c_exactly (hir : Hir) (n : Nat) : CompilerM ThompsonRef := do
+private def c_exactly (hir : Hir) (n : Nat) (states : States) : CompilerM (ThompsonRefStates states) := do
   if 0 < n then
-    let ⟨start, «end»⟩ ← c hir
-    let s ← (List.replicate (n-1) 0).foldlM (init := «end»)
-      (fun s _ => do
-        let ref ← c hir
-        patch s ref.start
-        pure ref.end)
-    pure ⟨start, s⟩
-  else c_empty
+    let ⟨(⟨start, «end»⟩, states'), _⟩ ← c hir states
+    let (⟨(s, states''), _⟩ : (StateIDStates' states states')) ←
+      (List.replicate (n-1) 0).foldlM (init := ⟨(«end», states'), by simp_all⟩)
+        (fun ⟨(s, states), _⟩ _ => do
+          let ⟨(ref, states), _⟩ ← c hir states
+          let states ← patch s ref.start states (by simp_all) (by simp_lte)
+          pure ⟨(ref.end, states), by and_intros <;> simp_lte⟩)
+    pure (ThompsonRefStates.mk start s states'' (by and_intros <;> simp_lte))
+  else c_empty states
 termination_by sizeOf hir + sizeOf n
 
 /-- embed `start` to `end` states in a possessive union,
     i.e. remove backtracking frames from stack if `end` state is reached
 -/
-private def c_possessive (tref : ThompsonRef) : CompilerM ThompsonRef := do
-  let union ← add_union
-  let fail ← add_fail
-  let eat ← add_eat (Unchecked.EatMode.ToLast 0)
-  let empty ← add_empty
+private def c_possessive (tref : ThompsonRef) (states : States)
+  (h1 : tref.start < states.val.size) (h2 : tref.end < states.val.size)
+    : CompilerM (ThompsonRefStates states) := do
+  let  ⟨(union, states), _⟩ ← add_union states
+  let  ⟨(fail, states), _⟩ ← add_fail states
+  let  ⟨(eat, states), _⟩ ← add_eat (Unchecked.EatMode.ToLast 0) states (by
+    simp [Unchecked.EatMode.nextOf])
+  let  ⟨(empty, states), _⟩ ← add_empty states
 
-  patch union tref.start
-  patch tref.«end» eat
-  patch union fail
-  patch eat fail
-  patch eat empty
-  pure ⟨union, empty⟩
+  let states ← patch union tref.start states (by simp_lte) (by simp_lte)
+  let states ← patch tref.«end» eat states (by simp_lte) (by simp_lte)
+  let states ← patch union fail states (by simp_lte) (by simp_lte)
+  let states ← patch eat fail states (by simp_lte) (by simp_lte)
+  let states ← patch eat empty states (by simp_lte) (by simp_lte)
+  pure (ThompsonRefStates.mk union empty states (by and_intros <;> simp_lte))
 
 private def is_possible_empty_repetition (hir : Hir) : Bool :=
   match hir with
@@ -262,187 +488,201 @@ private def get_possible_empty_capture_group (hir : Hir) : Option Nat :=
   | _ => none
 
 /-- Compile the given expression such that it may be matched `n` or more times -/
-private def c_at_least (hir : Hir) (n : Nat) (greedy : Bool) (possessive : Bool) : CompilerM ThompsonRef := do
+private def c_at_least (hir : Hir) (n : Nat) (greedy : Bool) (possessive : Bool) (states : States)
+    : CompilerM (ThompsonRefStates states) := do
   if n = 0 then
     /- compile x* as (x+)?, which preserves the correct preference order
         if x can match the empty string. -/
-    let compiled ← c hir
-     let plus ← (if greedy then add_union else add_union_reverse)
+    let ⟨(compiled, states), _⟩ ← c hir states
+    let ⟨(plus, states), _⟩ ← (if greedy then add_union states else add_union_reverse states)
 
-    patch compiled.end plus
-    patch plus compiled.start
+    let states ← patch compiled.end plus states (by simp_lte) (by simp_lte)
+    let states ← patch plus compiled.start states (by simp_lte) (by simp_lte)
 
-    let (states, groups) ← get
+    let groups ← get
     let groups := match (if greedy then get_possible_empty_capture_group hir else none) with
               | some g => groups.push g
               | none => groups
-    set (states, groups)
+    set groups
 
-    let question ← (if greedy then add_union else add_union_reverse)
-    let empty ← add_empty
-    patch question compiled.start
-    patch question empty
-    patch plus empty
+    let  ⟨(question, states), _⟩ ← (if greedy then add_union states else add_union_reverse states)
+    let  ⟨(empty, states), _⟩ ← add_empty states
+    let states ← patch question compiled.start states (by simp_lte) (by simp_lte)
+    let states ← patch question empty states (by simp_lte) (by simp_lte)
+    let states ← patch plus empty states (by simp_lte) (by simp_lte)
 
     if possessive then
-      c_possessive ⟨question, empty⟩
+      let t ← c_possessive ⟨question, empty⟩ states (by simp_lte) (by simp_lte)
+      pure (ThompsonRefStates.castLt t (by have ⟨_, _, _⟩ := t.property; simp_lte))
     else
-      pure ⟨question, empty⟩
+      pure (ThompsonRefStates.mk question empty states (by and_intros <;> simp_lte))
   else if n = 1 then
-    let compiled ← c hir
-    let union ← (if greedy then add_union else add_union_reverse)
+    let ⟨(compiled, states), _⟩ ← c hir states
+    let ⟨(union, states), _⟩ ← (if greedy then add_union states else add_union_reverse states)
 
-    let (states, groups) ← get
+    let groups ← get
     let groups := match (if greedy then get_possible_empty_capture_group hir else none) with
               | some g => groups.push g
               | none => groups
-    set (states, groups)
+    set groups
 
-    patch compiled.end union
-    patch union compiled.start
+    let states ← patch compiled.end union states (by simp_lte) (by simp_lte)
+    let states ← patch union compiled.start states (by simp_lte) (by simp_lte)
 
     if possessive then
-      c_possessive ⟨compiled.start, union⟩
+      let t ← c_possessive ⟨compiled.start, union⟩ states (by simp_lte) (by simp_lte)
+      pure (ThompsonRefStates.castLt t (by have ⟨_, _, _⟩ := t.property; simp_lte))
     else
-      pure ⟨compiled.start, union⟩
+      pure (ThompsonRefStates.mk compiled.start union states (by and_intros <;> simp_lte))
   else
-    let «prefix» ← c_exactly hir (n-1)
-    let last ← c hir
-    let union ← (if greedy then add_union else add_union_reverse)
+    let ⟨(«prefix», states), _⟩ ← c_exactly hir (n-1) states
+    let ⟨(last, states), _⟩ ← c hir states
+    let ⟨(union, states), _⟩ ← (if greedy then add_union states else add_union_reverse states)
 
-    patch «prefix».end last.start
-    patch last.end union
-    patch union last.start
+    let states ← patch «prefix».end last.start states (by simp_lte) (by simp_lte)
+    let states ← patch last.end union states (by simp_lte) (by simp_lte)
+    let states ← patch union last.start states (by simp_lte) (by simp_lte)
 
     if possessive then
-      c_possessive  ⟨«prefix».start, union⟩
+      let t ← c_possessive  ⟨«prefix».start, union⟩ states (by simp_lte) (by simp_lte)
+      pure (ThompsonRefStates.castLt t (by have ⟨_, _, _⟩ := t.property; simp_lte))
     else
-      pure ⟨«prefix».start, union⟩
+      pure (ThompsonRefStates.mk «prefix».start union states (by and_intros <;> simp_lte))
 termination_by sizeOf hir + sizeOf n + 1
 
 /-- Compile the given expression such that it matches at least `min` times,
     but no more than `max` times.-/
 private def c_bounded (hir : Hir) (min max : Nat) (greedy : Bool) (possessive : Bool)
-    : CompilerM ThompsonRef := do
-  if h : 0 < max then
-    let «prefix» ← c_exactly hir min
+  (states : States) : CompilerM (ThompsonRefStates states) := do
+  if 0 < max then
+    let ⟨(«prefix», states), _⟩  ← c_exactly hir min states
     if min = max then
       if possessive then
-        c_possessive «prefix»
+        let t ← c_possessive «prefix» states (by simp_lte) (by simp_lte)
+        pure (ThompsonRefStates.castLt t (by have ⟨_, _, _⟩ := t.property; simp_lte))
       else
-        pure «prefix»
+        pure (ThompsonRefStates.mk «prefix».start «prefix».end states (by and_intros <;> simp_lte))
     else
-      let empty ← add_empty
-      let prev_end ← (List.replicate (max-min) 0).foldlM (init := «prefix».end)
-        (fun prev_end _ => do
-          let compiled ← c hir
-          let union ← (if greedy then add_union else add_union_reverse)
+      let ⟨(empty, states'), _⟩ ← add_empty states
 
-          patch prev_end union
-          patch union compiled.start
+      let (⟨(prev_end, states''), _⟩ : (StateIDStates' states states')) ←
+        (List.replicate (max-min) 0).foldlM (init := ⟨(«prefix».end, states'),
+                                                       by and_intros <;> simp_lte⟩)
+          (fun ⟨(prev_end, states), _⟩ _ => do
+            let ⟨(compiled, states), _⟩ ← c hir states
+            let ⟨(union, states), _⟩ ←
+              (if greedy then add_union states else add_union_reverse states)
 
-          if possessive then
-            let union ← add_union
-            let fail ← add_fail
-            let eat ← add_eat (Unchecked.EatMode.ToLast 0)
+            let states ← patch prev_end union states (by simp_lte) (by simp_lte)
+            let states ← patch union compiled.start states (by simp_lte) (by simp_lte)
 
-            patch union fail
-            patch eat fail
-            patch eat empty
+            if possessive then
+              let ⟨(union, states), _⟩ ← add_union states
+              let ⟨(fail, states), _⟩ ← add_fail states
+              let ⟨(eat, states), _⟩ ← add_eat (Unchecked.EatMode.ToLast 0) states
+                (by simp [Unchecked.EatMode.nextOf])
 
-            pure compiled.end
-          else
-            patch union empty
-            pure compiled.end)
-      patch prev_end empty
-      pure ⟨«prefix».start, empty⟩
-  else c_empty
+              let states ← patch union fail states (by simp_lte) (by simp_lte)
+              let states ← patch eat fail states (by simp_lte) (by simp_lte)
+              let states ← patch eat empty states (by simp_lte) (by simp_lte)
+
+              pure ⟨(compiled.end, states), by and_intros <;> simp_lte⟩
+            else
+              let states ← patch union empty states (by simp_lte) (by simp_lte)
+              pure ⟨(compiled.end, states), by and_intros <;> simp_lte⟩)
+      let ⟨states'', _⟩ ← patch prev_end empty states'' (by simp_lte) (by simp_lte)
+      pure (ThompsonRefStates.mk «prefix».start empty states'' (by and_intros <;> simp_lte))
+  else c_empty states
 termination_by sizeOf hir + sizeOf min + sizeOf max
 
-private def c_back_ref (case_insensitive : Bool) (n : Nat) : CompilerM ThompsonRef := do
-  let backrefence ← add_backrefence case_insensitive n
-  let empty ← add_empty
-  patch backrefence empty
-  pure ⟨backrefence, empty⟩
+private def c_back_ref (case_insensitive : Bool) (n : Nat) (states : States)
+    : CompilerM (ThompsonRefStates states) := do
+  let ⟨(backrefence, states), _⟩ ← add_backrefence case_insensitive n states
+  let ⟨(empty, states), _⟩ ← add_empty states
+  let states ← patch backrefence empty states (by simp_lte) (by simp_lte)
+  pure (ThompsonRefStates.mk backrefence empty states (by and_intros <;> simp_lte))
 
-private def c_lookaround (look : Lookaround) : CompilerM ThompsonRef := do
+private def c_lookaround (look : Lookaround) (states : States)
+    : CompilerM (ThompsonRefStates states) := do
   match look with
   | .PositiveLookahead h =>
-    let compiled ← c h
-    let change_state ← add_change_state
-    let fail ← add_fail
-    let union ← add_union
-    let «end» ← add_empty
+    let ⟨(compiled, states), _⟩ ← c h states
+    let ⟨(change_state, states), _⟩ ← add_change_state states
+    let ⟨(fail, states), _⟩ ← add_fail states
+    let ⟨(union, states), _⟩ ← add_union states
+    let ⟨(«end», states), _⟩ ← add_empty states
 
-    patch compiled.end change_state
-    patch union compiled.start
-    patch change_state fail
-    patch change_state «end»
-    patch union fail
+    let states ← patch compiled.end change_state states (by simp_lte) (by simp_lte)
+    let states ← patch union compiled.start states (by simp_lte) (by simp_lte)
+    let states ← patch change_state fail states (by simp_lte) (by simp_lte)
+    let states ← patch change_state «end» states (by simp_lte) (by simp_lte)
+    let states ← patch union fail states (by simp_lte) (by simp_lte)
 
-    pure ⟨union, «end»⟩
+    pure (ThompsonRefStates.mk union «end» states (by and_intros <;> simp_lte))
   | .NegativeLookahead h =>
-    let compiled ← c h
-    let remove_state ← add_remove_state
-    let empty ← add_empty
-    let union ← add_union
-    let «end» ← add_empty
+    let ⟨(compiled, states), _⟩ ← c h states
+    let ⟨(remove_state, states), _⟩ ← add_remove_state states
+    let ⟨(empty, states), _⟩ ← add_empty states
+    let ⟨(union, states), _⟩ ← add_union states
+    let ⟨(«end», states), _⟩ ← add_empty states
 
-    patch compiled.end remove_state
-    patch remove_state empty
-    patch union compiled.start
-    patch empty «end»
-    patch union empty
+    let states ← patch compiled.end remove_state states (by simp_lte) (by simp_lte)
+    let states ← patch remove_state empty states (by simp_lte) (by simp_lte)
+    let states ← patch union compiled.start states (by simp_lte) (by simp_lte)
+    let states ← patch empty «end» states (by simp_lte) (by simp_lte)
+    let states ← patch union empty states (by simp_lte) (by simp_lte)
 
-    pure ⟨union, «end»⟩
+    pure (ThompsonRefStates.mk union «end» states (by and_intros <;> simp_lte))
   | .PositiveLookbehind length h =>
-    let next_char ← add_next_char length
-    let compiled ← c h
-    let «end» ← add_empty
+    let ⟨(next_char, states), _⟩ ← add_next_char length states
+    let ⟨(compiled, states), _⟩ ← c h states
+    let ⟨(«end», states), _⟩ ← add_empty states
 
-    patch next_char compiled.start
-    patch compiled.end «end»
+    let states ← patch next_char compiled.start states (by simp_lte) (by simp_lte)
+    let states ← patch compiled.end «end» states (by simp_lte) (by simp_lte)
 
-    pure ⟨next_char, «end»⟩
+    pure (ThompsonRefStates.mk  next_char «end» states (by and_intros <;> simp_lte))
   | .NegativeLookbehind length h =>
-    let next_char ← add_next_char length
-    let compiled ← c h
-    let remove_state ← add_remove_state
-    let empty ← add_empty
-    let union ← add_union
-    let «end» ← add_empty
+    let ⟨(next_char, states), _⟩ ← add_next_char length states
+    let ⟨(compiled, states), _⟩ ← c h states
+    let ⟨(remove_state, states), _⟩ ← add_remove_state states
+    let ⟨(empty, states), _⟩ ← add_empty states
+    let ⟨(union, states), _⟩ ← add_union states
+    let ⟨(«end», states), _⟩ ← add_empty states
 
-    patch next_char compiled.start
-    patch compiled.end remove_state
-    patch remove_state empty
-    patch union next_char
-    patch empty «end»
-    patch union empty
+    let states ← patch next_char compiled.start states (by simp_lte) (by simp_lte)
+    let states ← patch compiled.end remove_state states (by simp_lte) (by simp_lte)
+    let states ← patch remove_state empty states (by simp_lte) (by simp_lte)
+    let states ← patch union next_char states (by simp_lte) (by simp_lte)
+    let states ← patch empty «end» states (by simp_lte) (by simp_lte)
+    let states ← patch union empty states (by simp_lte) (by simp_lte)
 
-    pure ⟨union, «end»⟩
+    pure (ThompsonRefStates.mk union «end» states (by and_intros <;> simp_lte))
 termination_by sizeOf look
 
-private def c_repetition (rep : Repetition) : CompilerM ThompsonRef := do
+private def c_repetition (rep : Repetition) (_states : States)
+    : CompilerM (ThompsonRefStates _states) := do
   match rep with
   | .mk 0 (some 1) greedy false h => do
-      let union ← if greedy then add_union else add_union_reverse
-      let compiled ← c h
-      let empty ← add_empty
-      patch union compiled.start
-      patch union empty
-      patch compiled.end empty
-      pure ⟨union, empty⟩
+      let ⟨(union, states), _⟩ ← if greedy then add_union _states else add_union_reverse _states
+      let ⟨(compiled, states), _⟩ ← c h states
+      let ⟨(empty, states), _⟩ ← add_empty states
+      let states ← patch union compiled.start states (by simp_lte) (by simp_lte)
+      let states ← patch union empty states (by simp_lte) (by simp_lte)
+      let states ← patch compiled.end empty states (by simp_lte) (by simp_lte)
+      pure (ThompsonRefStates.mk union empty states (by and_intros <;> simp_lte))
   | .mk 0 (some 1) _ true h => do
-      let union ← add_union
-      let compiled ← c h
-      let eat ← add_eat (Unchecked.EatMode.Until 0)
-      let empty ← add_empty
-      patch union compiled.start
-      patch union empty
-      patch compiled.end eat
-      patch eat empty
-      patch eat empty
-      pure ⟨union, empty⟩
+      let ⟨(union, states), _⟩ ← add_union _states
+      let ⟨(compiled, states), _⟩ ← c h states
+      let ⟨(eat, states), _⟩ ← add_eat (Unchecked.EatMode.Until 0) states
+        (by simp [Unchecked.EatMode.nextOf])
+      let ⟨(empty, states), _⟩ ← add_empty states
+      let states ← patch union compiled.start states (by simp_lte) (by simp_lte)
+      let states ← patch union empty states (by simp_lte) (by simp_lte)
+      let states ← patch compiled.end eat states (by simp_lte) (by simp_lte)
+      let states ← patch eat empty states (by simp_lte) (by simp_lte)
+      let states ← patch eat empty states (by simp_lte) (by simp_lte)
+      pure (ThompsonRefStates.mk union empty states (by and_intros <;> simp_lte))
   | .mk min none greedy possessive sub => do
       let cannotMatchEmptyString : Bool :=
         match sub.properties.minimum_len with
@@ -450,50 +690,50 @@ private def c_repetition (rep : Repetition) : CompilerM ThompsonRef := do
         | none => false
       if min = 0 && cannotMatchEmptyString
       then
-        let union ← if greedy then add_union else add_union_reverse
-        let compiled ← c sub
-        patch union compiled.start
-        patch compiled.end union
-        pure ⟨union, union⟩
-      else c_at_least sub min greedy possessive
+        let ⟨(union, states), _⟩ ← if greedy then add_union _states else add_union_reverse _states
+        let ⟨(compiled, states), _⟩ ← c sub  states
+        let states ← patch union compiled.start states (by simp_lte) (by simp_lte)
+        let states ← patch compiled.end union states (by simp_lte) (by simp_lte)
+        pure (ThompsonRefStates.mk union union states (by and_intros <;> simp_lte))
+      else c_at_least sub min greedy possessive _states
   | .mk min (some max) greedy possessive sub =>
-      if min ≤ max then c_bounded sub min max greedy possessive else c_empty
+      if min ≤ max then c_bounded sub min max greedy possessive _states else c_empty _states
 termination_by sizeOf rep
 
-private def c (hir : Hir) : CompilerM ThompsonRef :=
-  have : sizeOf hir.kind < sizeOf hir := Hir.sizeOfKindOfHir hir
-  match h : hir.kind with
-  | .Empty => c_empty
-  | .Literal c => c_literal c
-  | .Class (.Unicode cls) => c_unicode_class cls
-  | .Look look => c_look look
-  | .Lookaround look =>
-    have : sizeOf look < sizeOf hir.kind := by simp [h]
-    c_lookaround look
-  | .BackRef f n => c_back_ref f n
-  | .Repetition rep =>
-    have : sizeOf rep < sizeOf hir.kind := by simp [h]
-    c_repetition rep
-  | .Capture cap =>
-    have : sizeOf cap < sizeOf hir.kind := by simp [h]
-    c_cap cap
-  | .Concat items =>
-    have : sizeOf items < sizeOf hir.kind := by simp [h]
-    c_concat items
-  | .Alternation sub =>
-    have : sizeOf sub < sizeOf hir.kind := by simp [h]
-    c_alt_iter sub
+private def c_cap (hir : Capture) (states : States) : CompilerM (ThompsonRefStates states) := do
+  match hir with
+    | .mk pattern_id _ sub =>
+      let ⟨(start, states), _⟩ ← c_cap' Capture.Role.Start pattern_id (pattern_id * 2) states
+      let ⟨(«inner», states), _⟩ ← c sub states
+      let ⟨(«end», states), _⟩ ← c_cap' Capture.Role.End pattern_id (pattern_id * 2 + 1) states
+      let states ← patch start inner.start states (by simp_lte) (by simp_lte)
+      let states ← patch inner.end «end» states (by simp_lte) (by simp_lte)
+      pure (ThompsonRefStates.mk start «end» states (by and_intros <;> simp_lte))
 termination_by sizeOf hir
 
-private def c_cap (hir : Capture) : CompilerM ThompsonRef := do
-  match hc : hir with
-    | .mk pattern_id name sub =>
-      let start ← c_cap' Capture.Role.Start pattern_id (pattern_id * 2)
-      let inner ← c sub
-      let «end» ← c_cap' Capture.Role.End pattern_id (pattern_id * 2 + 1)
-      patch start inner.start
-      patch inner.end «end»
-      pure ⟨start, «end»⟩
+private def c (hir : Hir) (_states : States) : CompilerM (ThompsonRefStates _states) :=
+  have : sizeOf hir.kind < sizeOf hir := Hir.sizeOfKindOfHir hir
+  match h : hir.kind with
+  | .Empty => c_empty _states
+  | .Literal c => c_literal c _states
+  | .Class (.Unicode cls) => c_unicode_class cls _states
+  | .Look look => c_look look _states
+  | .Lookaround look =>
+    have : sizeOf look < sizeOf hir.kind := by simp [h]
+    c_lookaround look _states
+  | .BackRef f n => c_back_ref f n _states
+  | .Repetition rep =>
+    have : sizeOf rep < sizeOf hir.kind := by simp [h]
+    c_repetition rep _states
+  | .Capture cap =>
+    have : sizeOf cap < sizeOf hir.kind := by simp [h]
+    c_cap cap _states
+  | .Concat items =>
+    have : sizeOf items < sizeOf hir.kind := by simp [h]
+    c_concat items _states
+  | .Alternation sub =>
+    have : sizeOf sub < sizeOf hir.kind := by simp [h]
+    c_alt_iter sub _states
 termination_by sizeOf hir
 
 end
@@ -507,23 +747,25 @@ private def startsWithStart (hir : Hir) : Bool :=
   | _ => false
 
 /-- Compile the HIR expression given. -/
-private def compile' (anchored : Bool) (expr : Hir) : CompilerM PUnit := do
-  let unanchored_prefix ←
-    if anchored then c_empty
-    else c_repetition <| Repetition.mk 0 none false false (dot Dot.AnyChar)
-  let one ← c_cap (Capture.mk 0 none expr)
-  let match_state_id ← add_match 0
-  patch one.end match_state_id
-  patch unanchored_prefix.end one.start
+private def compile' (anchored : Bool) (expr : Hir) : CompilerM States := do
+  let states : States := ⟨#[], by simp_all⟩
+  let ⟨(unanchored_prefix, states), _⟩ ←
+    if anchored then c_empty states
+    else c_repetition (Repetition.mk 0 none false false (dot Dot.AnyChar)) states
+  let ⟨(one, states), _⟩ ← c_cap (Capture.mk 0 none expr) states
+  let ⟨(match_state_id, states), _⟩ ← add_match 0 states
+  let states ← patch one.end match_state_id states (by simp_lte) (by simp_lte)
+  patch unanchored_prefix.end one.start states (by simp_lte) (by simp_lte)
 
 /-- Compile the HIR expression given. -/
 def compile (config : Config := default) (flavor : Syntax.Flavor) (expr : Hir)
     : Except String Checked.NFA := do
   let unanchored_prefix_simulation := expr.containsLookaround || config.unanchored_prefix_simulation
   let anchored := !config.unanchored_prefix || startsWithStart expr || unanchored_prefix_simulation
-  let (_, (states, groups)) ← compile' anchored expr (#[], #[])
-  let nfa ← NFA.toCkecked ⟨states, Unchecked.toSlots states, 0, 0⟩
+  let (states, groups) ← compile' anchored expr #[]
+  let nfa ← NFA.toCkecked ⟨states.val, Unchecked.toSlots states, 0, 0⟩
               (match flavor with | Syntax.Flavor.Pcre => groups | _ => #[])
+              states.property
   Except.ok {nfa with unanchored_prefix_in_backtrack :=
                   !startsWithStart expr && unanchored_prefix_simulation
             }
